more work on splittable; augmented Compose to work with syntaxes

MergeSemTc/Compose.thy
@@ -22,85 +22,165 @@ for the Views will need to be ordered *)
 
 *)
 
-
+(* TODO: make this n-ary instead of binary? *)
 class Comp = Mergeableb + Splittableb +
-  fixes sem1 :: "('a :: Splittable) \<Rightarrow> 'a"
-  fixes sem2 :: "'a \<Rightarrow> 'a"
-  fixes sem1_name :: "'a itself \<Rightarrow> char list"
-  fixes sem2_name :: "'a itself \<Rightarrow> char list"
-  assumes Proj_Wf1 : "sem1_name t \<in> projs_names (t)"
-  assumes Proj_Wf2 : "sem2_name t \<in> projs_names (t)"
-  assumes Sem1_Dom : "x \<in> (sdom (sem1_name t)) \<Longrightarrow> sem1 x \<in> (sdom (sem1_name t))"
-  assumes Sem2_Dom : "x \<in> (sdom (sem2_name t)) \<Longrightarrow> sem2 x \<in> (sdom (sem2_name t))"
+  (* idea: we call these with
+     - an 'a \<in> syn1 representing the syntax
+     - an 'a \<in> st1 representing the state *)
+  fixes sem1 :: "('a :: Splittable) \<Rightarrow> 'a \<Rightarrow> 'a"
+  fixes sem2 :: "'a \<Rightarrow> 'a \<Rightarrow> 'a"
+
+  fixes st1_name :: "'a itself \<Rightarrow> char list"
+  fixes st2_name :: "'a itself \<Rightarrow> char list"
+  fixes syn1_name :: "'a itself \<Rightarrow> char list"
+  fixes syn2_name :: "'a itself \<Rightarrow> char list"
+
+  assumes Proj_Wf_St1 : "st1_name t \<in> projs_names (t)"
+  assumes Proj_Wf_St2 : "st2_name t \<in> projs_names (t)"
+  assumes Proj_Wf_Syn1 : "syn1_name t \<in> projs_names (t)"
+  assumes Proj_Wf_Syn2 : "syn2_name t \<in> projs_names (t)"
+
+  assumes Sem1_Dom : "st \<in> (sdom (sem1_name t)) \<Longrightarrow>
+                      syn \<in> (sdom (syn1_name t)) \<Longrightarrow>
+                      sem1 syn st \<in> (sdom (sem1_name t))"
+  assumes Sem2_Dom : "st \<in> (sdom (sem2_name t)) \<Longrightarrow>
+                      syn \<in> (sdom (syn1_name t)) \<Longrightarrow>
+                      sem2 syn st \<in> (sdom (sem2_name t))"
+
+  assumes Sem1_Mono : "syn \<in> (sdom (syn1_name t)) \<Longrightarrow>
+                       syn' \<in> (sdom (syn1_name t)) \<Longrightarrow>
+                       syn <[ syn' \<Longrightarrow>
+                       sem1 syn st <[ sem1 syn' st"
+
+  assumes Sem2_Mono : "syn \<in> (sdom (syn2_name t)) \<Longrightarrow>
+                       syn' \<in> (sdom (syn2_name t)) \<Longrightarrow>
+                       syn <[ syn' \<Longrightarrow>
+                       sem2 syn st <[ sem2 syn' st"
+
+  (* TODO: are these axioms enough? *)
   assumes Pres :
-  "x1 \<in> (sdom (sem1_name t)) \<Longrightarrow> x2 \<in> (sdom (sem2_name t)) \<Longrightarrow>
-   has_sup {x1, x2} \<Longrightarrow>
-   has_sup {sem1 x1, sem2 x2}"
+  "st1 \<in> (sdom (st1_name t)) \<Longrightarrow>
+   st2 \<in> (sdom (st2_name t)) \<Longrightarrow>
+   syn1 \<in> (sdom (syn1_name t)) \<Longrightarrow>
+   syn2 \<in> (sdom (syn2_name t)) \<Longrightarrow>
+   has_sup {st1, st2} \<Longrightarrow>
+   has_sup {syn1, syn2} \<Longrightarrow>
+   has_sup {sem1 syn1 st1, sem2 syn2 st2}"
 
-definition cdom_l :: "('a :: Comp) set" where
-"cdom_l = (sdom (sem1_name (TYPE('a))))"
+definition cst_l :: "('a :: Comp) set" where
+"cst_l = (sdom (st1_name (TYPE('a))))"
 
-definition cdom_r :: "('a :: Comp) set" where
-"cdom_r = (sdom (sem2_name (TYPE('a))))"
+definition cstprj_l :: "'a :: Comp \<Rightarrow> 'a" where
+"cstprj_l = sprj (st1_name (TYPE('a)))"
+
+definition cst_r :: "('a :: Comp) set" where
+"cst_r = (sdom (st2_name (TYPE('a))))"
+
+definition cstprj_r :: "'a :: Comp \<Rightarrow> 'a" where
+"cstprj_r = sprj (st2_name (TYPE('a)))"
+
+definition csyn_l :: "('a :: Comp) set" where
+"csyn_l = (sdom (syn1_name (TYPE('a))))"
+
+definition csynprj_l :: "'a :: Comp \<Rightarrow> 'a" where
+"csynprj_l = sprj (syn1_name (TYPE('a)))"
+
+definition csyn_r :: "('a :: Comp) set" where
+"csyn_r = (sdom (syn2_name (TYPE('a))))"
+
+definition csynprj_r :: "'a :: Comp \<Rightarrow> 'a" where
+"csynprj_r = sprj (syn2_name (TYPE('a)))"
 
 
-typedef (overloaded) 'a cdom1t = "cdom_l :: ('a :: Comp) set"
+typedef (overloaded) 'a cst_lt = "cst_l :: ('a :: Comp) set"
 proof(-)
 
-  obtain d and f where Hdf : "Some (d, f) = map_of (projs :: ('a projs_t)) (sem1_name (TYPE('a)))"
-      using Proj_Wf1[of "(TYPE('a))"]
+  obtain d and f where Hdf : "Some (d, f) = map_of (projs :: ('a projs_t)) (st1_name (TYPE('a)))"
+      using Proj_Wf_St1[of "(TYPE('a))"]
             projs_distinct'[of "projs :: 'a projs_t"]
       by(auto simp add:projs_names_def)
     
 
-  hence "(sem1_name (TYPE('a)), d, f) \<in> set (projs :: 'a projs_t)"
+  hence "(st1_name (TYPE('a)), d, f) \<in> set (projs :: 'a projs_t)"
     by(auto intro:map_of_SomeD)
 
   hence "\<bottom> \<in> d" by (auto elim:projs_bot)
 
-  thus ?thesis using Hdf by(cases "map_of (projs :: 'a projs_t) (sem1_name (TYPE('a)))"; auto simp add:cdom_l_def sdom_def sdom'_def)
+  thus ?thesis using Hdf by(cases "map_of (projs :: 'a projs_t) (st1_name (TYPE('a)))"; auto simp add:cst_l_def sdom_def sdom'_def)
 qed
 
-typedef (overloaded) 'a cdom2t = "cdom_r :: ('a :: Comp) set"
+typedef (overloaded) 'a cst_rt = "cst_r :: ('a :: Comp) set"
 proof(-)
-  obtain d and f where Hdf : "Some (d, f) = map_of (projs :: ('a projs_t)) (sem2_name (TYPE('a)))"
-      using Proj_Wf2[of "(TYPE('a))"]
+
+  obtain d and f where Hdf : "Some (d, f) = map_of (projs :: ('a projs_t)) (st2_name (TYPE('a)))"
+      using Proj_Wf_St2[of "(TYPE('a))"]
             projs_distinct'[of "projs :: 'a projs_t"]
       by(auto simp add:projs_names_def)
     
 
-  hence "(sem2_name (TYPE('a)), d, f) \<in> set (projs :: 'a projs_t)"
+  hence "(st2_name (TYPE('a)), d, f) \<in> set (projs :: 'a projs_t)"
     by(auto intro:map_of_SomeD)
 
   hence "\<bottom> \<in> d" by (auto elim:projs_bot)
 
-  thus ?thesis using Hdf by(cases "map_of (projs :: 'a projs_t) (sem2_name (TYPE('a)))"; auto simp add:cdom_r_def sdom_def sdom'_def)
+  thus ?thesis using Hdf by(cases "map_of (projs :: 'a projs_t) (st2_name (TYPE('a)))"; auto simp add:cst_r_def sdom_def sdom'_def)
 qed
+
+typedef (overloaded) 'a csyn_lt = "csyn_l :: ('a :: Comp) set"
+proof(-)
+
+  obtain d and f where Hdf : "Some (d, f) = map_of (projs :: ('a projs_t)) (syn1_name (TYPE('a)))"
+      using Proj_Wf_Syn1[of "(TYPE('a))"]
+            projs_distinct'[of "projs :: 'a projs_t"]
+      by(auto simp add:projs_names_def)
+    
+
+  hence "(syn1_name (TYPE('a)), d, f) \<in> set (projs :: 'a projs_t)"
+    by(auto intro:map_of_SomeD)
+
+  hence "\<bottom> \<in> d" by (auto elim:projs_bot)
+
+  thus ?thesis using Hdf by(cases "map_of (projs :: 'a projs_t) (syn1_name (TYPE('a)))"; auto simp add:csyn_l_def sdom_def sdom'_def)
+qed
+
+typedef (overloaded) 'a csyn_rt = "csyn_r :: ('a :: Comp) set"
+proof(-)
+
+  obtain d and f where Hdf : "Some (d, f) = map_of (projs :: ('a projs_t)) (syn2_name (TYPE('a)))"
+      using Proj_Wf_Syn2[of "(TYPE('a))"]
+            projs_distinct'[of "projs :: 'a projs_t"]
+      by(auto simp add:projs_names_def)
+    
+
+  hence "(syn2_name (TYPE('a)), d, f) \<in> set (projs :: 'a projs_t)"
+    by(auto intro:map_of_SomeD)
+
+  hence "\<bottom> \<in> d" by (auto elim:projs_bot)
+
+  thus ?thesis using Hdf by(cases "map_of (projs :: 'a projs_t) (syn2_name (TYPE('a)))"; auto simp add:csyn_r_def sdom_def sdom'_def)
+qed
+
 
 (*
 typedef (overloaded) 'a dom2 = "cdom_r :: ('a :: Comp) set"
 *)
 (* parallel composition *)
-definition pcomp :: "('a :: Comp) \<Rightarrow> 'a" where
-"pcomp x =
-  [^ [^ sem1 x, sem2 x ^], x ^]"
+definition pcomp :: "('a :: Comp) \<Rightarrow> 'a \<Rightarrow> 'a" where
+"pcomp syn st =
+  [^ [^ sem1 (csynprj_l syn) (cstprj_l st), sem2 (csynprj_r syn) (cstprj_r st) ^], st ^]"
 
-definition pcomp' :: "('a :: Comp) \<Rightarrow> 'a" where
-"pcomp' x =
-  [^ [^ sem2 x, sem1 x ^], x ^]"
+definition pcomp' :: "('a :: Comp) \<Rightarrow> 'a \<Rightarrow> 'a" where
+"pcomp' syn st =
+  [^ [^ sem2 (csynprj_r syn) (cstprj_r st), sem1 (csynprj_l syn) (cstprj_l st) ^], st ^]"
 
 (* "real" parallel semantics, which may contain more information *)
-definition pcomp_real :: "('a :: Comp) \<Rightarrow> 'a" where
-"pcomp_real x =
-  [^ sem1 x, [^ sem2 x, x ^]^]"
+definition pcomp_real :: "('a :: Comp) \<Rightarrow> 'a \<Rightarrow> 'a" where
+"pcomp_real syn st =
+  [^ sem1 (csynprj_l syn) (cstprj_l st), [^ sem2 (csynprj_r syn) (cstprj_r st), st ^]^]"
 
-definition pcomp_real' :: "('a :: Comp) \<Rightarrow> 'a" where
-"pcomp_real' x =
-  [^ sem2 x, [^ sem1 x, x ^]^]"
+definition pcomp_real' :: "('a :: Comp) \<Rightarrow> 'a \<Rightarrow> 'a" where
+"pcomp_real' syn st =
+  [^ sem2 (csynprj_r syn) (cstprj_r st), [^ sem1 (csynprj_l syn) (cstprj_l st), st ^]^]"
 
-
-(* next: extend this with syntaxes
-   idea: we now have 4 domains. syntax1, syntax2, semantics1, semantics2
-   6, if we count full syntax and full semantics *)
 
 end
